\begin{enumerate}[leftmargin=2cm,labelsep=.5cm,label=\bf\arabic*.]
\item \textit{Part 1:}
\begin{enumerate}
\item $t(2) = 7, \quad t(3) = 11, \quad t(4) = 15$
\item $t(2) = 3, \quad t(3) = 6,  \quad t(4) = 10$
\item $t(2) = 1, \quad t(3) = 3,  \quad t(4) = 7$
\item $t(2) = 6, \quad t(3) = 15, \quad t(4) = 31$\\[2mm]
\end{enumerate}
\textit{Part 2:}\\
$t(3) = 3, \quad t(4) = 5, \quad t(5) = 11$\\[1cm]

\item
\begin{enumerate}
\item $
\begin{aligned}[t]
t(n) - 5t(n-1) + 4t(n-2) &= 0 & t_1 \rightarrow c_1(1)^1 + c_2(4)^1 &= 2 \\
r^2 - 5r + 4 &= 0             & t_2 \rightarrow c_1(1)^2 + c_2(4)^2 &= -1 \\
r &= 1, 4                     & c_1 + 4c_2 &= 2 \\
&                             & c_1 + 16c_2 &= -1 \\[2mm]
c_1 &= 3, \quad c_2 = -\frac{1}{4}  & & \\
t_n &= 3(1)^n -\frac{1}{4}(4)^n \\[1cm]
\end{aligned} $


\item $
\begin{aligned}[t]
t(n) - 2t(n-1) - 8t(n-2) &= 0 & t_1 \rightarrow c_1(-2)^1 + c_2(4)^1 &= 1 \\
r^2 - 2r - 8 &= 0             & t_2 \rightarrow c_1(-2)^2 + c_2(4)^2 &= 0 \\
r &= -2, 4                    & -2c_1 + 4c_2 &= 1 \\
&                             & 4c_1 + 16c_2 &= 0 \\[2mm]
c_1 &= -\frac{1}{3}, \quad c_2 = \frac{1}{12}  & & \\
t_n &= -\frac{1}{3}(-2)^n + \frac{1}{12}(4)^n \\[1cm]
\end{aligned} $

\item $
\begin{aligned}[t]
t(n) - 6t(n-1) + 9t(n-2) &= 0 & t_1 \rightarrow 3^1(c_1 + c_2(1)) &= 3 \\
r^2 - 6r + 9 &= 0             & t_2 \rightarrow 3^2(c_1 + c_2(2)) &= 2 \\
r &= 3                        & 3c_1 + 3c_2 &= 3 \\
&                             & 9c_1 + 18c_2 &= 2 \\[2mm]
c_1 &= \frac{16}{9}, \quad c_2 = -\frac{7}{9}  & & \\
t_n &= 3^n\left(\frac{16}{9} - \frac{7}{9}n\right) \\[1cm]
\end{aligned} $

\item $
\begin{aligned}[t]
t(n) + 5t(n-1) + 6t(n-2) &= 0 & t_1 \rightarrow c_1(-3)^1 + c_2(-2)^1 &= 1 \\
r^2 + 5r + 6 &= 0             & t_2 \rightarrow c_1(-3)^2 + c_2(-2)^2 &= -4 \\
r &= -3, -2                   & -3c_1 - 2c_2 &= 1 \\
&                             & 9c_1 + 4c_2 &= -4 \\[2mm]
c_1 &= -\frac{2}{3}, \quad c_2 = \frac{1}{2}  & & \\
t_n &= -\frac{2}{3}(-3)^n + \frac{1}{2}(-2)^n \\[1cm]
\end{aligned} $

\item $
\begin{aligned}[t]
t(n) + 2t(n-1) + t(n-2) &= 0  & t_1 \rightarrow -1^1(c_1 + c_2(1)) &= 3 \\
r^2 + 2r + 1 &= 0             & t_2 \rightarrow -1^2(c_1 + c_2(2)) &= 3 \\
r &= -1                       & -c_1 - c_2 &= 3 \\
&                             & c_1 + 2c_2 &= 3 \\[2mm]
c_1 &= -9, \quad c_2 = 6  & & \\
t_n &= -1^n(-9 + 6n) \\[1cm]
\end{aligned} $

\item $
\begin{aligned}[t]
t(n) - 25t(n-2) &= 0          & t_1 \rightarrow c_1(-5)^1 + c_2(5)^1 &= -1 \\
r^2 - 25 &= 0                 & t_2 \rightarrow c_1(-5)^2 + c_2(5)^2 &= 1 \\
r &= -5, 5                    & -5c_1 + 5c_2 &= -1 \\
&                             & 25c_1 + 25c_2 &= 1 \\[2mm]
c_1 &= \frac{3}{25}, \quad c_2 = -\frac{2}{25}  & & \\
t_n &= \frac{3}{25}(-5)^n -\frac{2}{25}(5)^n \\[1cm]
\end{aligned} $
\end{enumerate}

\item
\begin{enumerate}
\item $
\begin{aligned}[t]
a_n + 4a_{n-2} &= 0                & a_0 \rightarrow 2^0(c_1\cos{0} + c_2\sin{0}) &= 1 \\
r^2 + 4 &= 0                       & a_1 \rightarrow 2^1\left(c_1\cos{\frac{\pi}{2}} + c_2\sin{\frac{\pi}{2}}\right) &= 0 \\
r &= 0 \pm 2\mathrm{i}             & & \\
d &= \sqrt{0^2 + 2^2} = 2 & & \\
\theta &= \arctan\left(\frac{2}{0}\right) = \frac{\pi}{2} & & \\[2mm]
c_1 &= 1, \quad c_2 = 0 & & \\
a_n &= 2^n\left(\cos{\left(\frac{\pi}{2}n\right)}\right)\\[1cm]
\end{aligned} $

\item $
\begin{aligned}[t]
a_n - a_{n-1} + a_{n-2} &= 0       & a_0 \rightarrow c_1\cos{0} + c_2\sin{0} &= 0 \\
r^2 - r + 1 &= 0                   & a_1 \rightarrow c_1\cos{\frac{\pi}{3}} + c_2\sin{\frac{\pi}{3}}\right &= 1 \\
r &= \frac{1}{2} \pm \frac{\sqrt{3}}{2}\mathrm{i} & & \\
d &= \sqrt{\left(\frac{1}{2}\right)^2 + \left(\frac{\sqrt{3}}{2}\right)^2} = 1 \\
\theta &= \arctan\left(\sqrt{3}\right) = \frac{\pi}{3} & & \\[2mm]
c_1 &= 0, \quad c_2 = \frac{2}{\sqrt{3}} & & \\
a_n &= \frac{2}{\sqrt{3}}\sin{\left(\frac{\pi}{3}n\right)}\\[1cm]
\end{aligned} $



\item $
\begin{aligned}[t]
a_n - a_{n-1} - a_{n-2} &= 0                & a_0 \rightarrow c_1 + c_2 &= 0 \\
r^2 - r - 1 &= 0                            & a_1 \rightarrow c_1\left(\frac{1+\sqrt{5}}{2}\right)^1 + c_2\left(\frac{1-\sqrt{5}}{2}\right)^1 &= 1 \\
r &= \frac{1\pm\sqrt{5}}{2}                 & c_1 + c_2 &= 0 \\
&                                           & c_1\left(\frac{1+\sqrt{5}}{2}\right) + c_2\left(\frac{1-\sqrt{5}}{2}\right) &= 1 \\[2mm]
c_1 &= \frac{1}{\sqrt{5}} , \quad c_2 = -\frac{1}{\sqrt{5}}    & & \\
a_n &= \frac{1}{\sqrt{5}}\left[\left(\frac{1+\sqrt{5}}{2}\right)^n - \left(\frac{1-\sqrt{5}}{2}\right)^n\right]\\[1cm]
\end{aligned} $
\end{enumerate}

\item
\begin{enumerate}
\item $
\begin{aligned}[t]
S(n) \rightarrow 1+3+5+...+(2n-1)&=n^2\\
S(1) \rightarrow (2(1)-1)&=1^2\\
1&=1\\[5mm]
S(k) \rightarrow 1+3+5+...+(2k-1)&=k^2\\
S(k+1) \rightarrow 1+3+5+...+(2k-1) + 2(k+1)-1 &=(k+1)^2\\[5mm]
k^2+2(k+1)-1 &=(k+1)^2\\
k^2+2k+1 &=(k+1)^2\\
(k+1)(k+1)&=(k+1)^2\\[1cm]
\end{aligned} $

\item $
\begin{aligned}[t]
S(n) \rightarrow 1^2+2^2+3^2+...+n^2 &= \frac{n(n+1)(2n+1)}{6}\\
S(1) \rightarrow 1^2&=\frac{1(1+1)(2(1)+1)}{6}\\
1^2&=\frac{1(2)(3)}{6}\\
1=\frac{6}{6}&=1\\[5mm]
S(k) \rightarrow 1^2+2^2+3^2+...+k^2 &= \frac{k(k+1)(2k+1)}{6}\\
S(k+1) \rightarrow 1^2+2^2+3^2+...+k^2 +(k+1)^2 &= \frac{(k+1)(k+2)(2k+3)}{6}\\[5mm]
1^2+2^2+3^2+...+k^2 +(k+1)^2 &= \frac{k(k+1)(2k+1)}{6} + (k+1)^2\\
&=\frac{k(k+1)(2k+1)+6(k+1)^2}{6}\\
&=\frac{(k+1)\left[k(2k+1)+6(k+1)\right]}{6}\\
&=\frac{(k+1)(2k^2+7k+6)}{6}\\
&= \frac{(k+1)(k+2)(2k+3)}{6}
\end{aligned} $
\end{enumerate}

\end{enumerate}
